% theorem statement
If $m \in \mathbb{N}$ is even, then $m^2$ is even.

% proof
We will use induction on $m$.

The first base case, $m=0$ is trivial.

The second base case, $m=1$ is also trivial.

For $m = k+2$, based on the fact that $k+2$ is even, we can show that $k$ is even.

Hence, the induction hypothesis gives us that $k^2$ is even.

But we know that if $k^2$ is even, we have a natural number $l$ such that $k^2 = 2l$.

Combining this, we show that $(k+2)^2 = k^2 + 4k + 4 = 2l + 4k + 4 = 2(l+2k+2)$.

Therefore, $(k+2)^2$ is even.